Fix overflow errors (see #45).

src/dafny/beacon/Helpers.dfy
@@ -27,23 +27,82 @@ module BeaconHelpers {
 
     /**
      *  The epoch of a slot.
+     *
+     *  @param  slot    A slot.
+     *  @returns        The epoch of the slot.
      */
     function method compute_epoch_at_slot(slot: Slot) : Epoch
     {
         (slot / SLOTS_PER_EPOCH) as Epoch
     }
 
+    /**
+     *  Slot number at start of an epoch.
+     *  
+     *  @param  epoch   An epoch.
+     *  @returns        The slot number at the start of `epoch`.
+     *  @link{https://github.com/ethereum/eth2.0-specs/blob/dev/specs/phase0/beacon-chain.md#compute_start_slot_at_epoch}
+     */
+    function method compute_start_slot_at_epoch(epoch: Epoch) : Slot
+        requires epoch as int * SLOTS_PER_EPOCH as int < 0x10000000000000000    // report
+    {
+        epoch * SLOTS_PER_EPOCH as Slot
+    }
+
+    /**
+     *  @param  state   A beacon state.
+     *  @returns        The epoch of the state's slot.
+     */
     function method get_current_epoch(state: BeaconState) : Epoch 
     {
         compute_epoch_at_slot(state.slot)
     }
 
+    /**
+     *  @param  state   A beacon state.
+     *  @returns        Epoch before state's epoch and 0 is state's epoch is 0.
+     */
     function method get_previous_epoch(state: BeaconState) : Epoch 
     {
         var e := get_current_epoch(state);
         //  max(0, e - 1)
         if e > 0 then e - 1 else e 
     }
+
+    /**
+     *  The block root at the start of an epoch.
+     *
+     *  @param  state   A beacon state.
+     *  @param  epoch   A recent epoch (must be tracked in state.block_roots).
+     *  @returns        The block root at the beginning of epoch. 
+     *  @link{https://github.com/ethereum/eth2.0-specs/blob/dev/specs/phase0/beacon-chain.md#get_block_root}
+     *  
+     */
+    function method get_block_root(state: BeaconState, epoch: Epoch) : Root    
+        requires state.slot as int + SLOTS_PER_HISTORICAL_ROOT as int < 0x10000000000000000 //    report overflow
+        requires epoch as int * SLOTS_PER_EPOCH as int < 0x10000000000000000    // report
+        requires compute_start_slot_at_epoch(epoch) < state.slot <= compute_start_slot_at_epoch(epoch) + SLOTS_PER_HISTORICAL_ROOT  //  report 
+    { 
+        var e := compute_start_slot_at_epoch(epoch);
+        get_block_root_at_slot(state, e)
+    }
+    
+    /**
+     *  The block root at the start of a given (recent) slot.
+     *
+     *  @param  state   A beacon state.
+     *  @param  slot    A recent slot (must be tracked in state.block_roots).
+     *  @returns        The block root at (a recent) slot. 
+     *  @link{https://github.com/ethereum/eth2.0-specs/blob/dev/specs/phase0/beacon-chain.md#get_block_root_at_slot}
+     *  
+     */
+    function method get_block_root_at_slot(state: BeaconState, slot: Slot) : Root
+        requires slot as int + SLOTS_PER_HISTORICAL_ROOT as int < 0x10000000000000000 //    report overflow
+        requires slot < state.slot <= slot + SLOTS_PER_HISTORICAL_ROOT
+    {
+        state.block_roots[slot % SLOTS_PER_HISTORICAL_ROOT]
+    }
+    
     
 
 }
